rocq-osiris/theories/semantics/run.v
@@ -49,7 +49,7 @@ Fixpoint confluent_step {A E} (σ : store) (m : micro A E) : option (config A E)
   (* Final micros do not step *)
   | Ret _ | Throw _ | Crash => None
   (* Most side effects are not confluent *)
-  | Stop (CFlip | CLoad | CExchange | CCAS | CPerf | CResume | CWrap | CFork | CJoin) _ _ => None
+  | Stop (CFlip | CLoad | CExchange | CCAS | CFAA | CPerf | CResume | CWrap | CFork | CJoin) _ _ => None
   (* [CEval], [CLoop], [CAlloc], [Handle] have only one way to reduce *)
   | Stop CEval (η, e) k => Some (σ, try2 (pre_eval η e) k)
   | Stop CLoop (η, x, i1, i2, e) k => Some (σ, try2 (loop η x i1 i2 e) k)
@@ -128,6 +128,7 @@ Fixpoint stepto {A E} (σ : store) (m : micro A E) {struct m} : step_result A E 
   | Stop CLoad l k => Step [step_load σ l k]
   | Stop CExchange (l, v') k => Step [step_exchange σ l v' k]
   | Stop CCAS (l, seen, v') k => Step [step_cas σ l seen v' k]
+  | Stop CFAA (l, i) k => Step [step_faa σ l i k]
   | Stop CResume (l, o) k => Step [step_resume σ l o k]
   | Stop CWrap (true, l, η, bs) k => Step [step_wrap σ l η bs (fresh (dom σ)) k]
   | Stop CWrap (false, l, η, bs) k => Step [step_shallow_wrap σ l η bs (fresh (dom σ)) k]
@@ -366,6 +367,7 @@ Fixpoint string_of_expr (e : expr) : string :=
   | EStore e1 e2 => "EStore(" ++ string_of_expr e1 ++ ", " ++ string_of_expr e2 ++ ")"
   | EExchange e1 e2 => "EExchange(" ++ string_of_expr e1 ++ ", " ++ string_of_expr e2 ++ ")"
   | ECAS e1 e2 e3 => "ECAS(" ++ string_of_expr e1 ++ ", " ++ string_of_expr e2 ++ ", " ++ string_of_expr e3 ++ ")"
+  | EFAA e1 e2 => "EFAA(" ++ string_of_expr e1 ++ ", " ++ string_of_expr e2 ++ ")"
   | EIgnore e => "EIgnore(" ++ string_of_expr e ++ ")"
   | EFork e1 e2 => "EFork(" ++ string_of_expr e1 ++ ", " ++ string_of_expr e2 ++ ")"
   | EJoin e => "EFork(" ++ string_of_expr e ++ ")"
@@ -448,6 +450,7 @@ Definition string_of_code {X Y Z} (c : code X Y Z) : string :=
   | CLoad => "CLoad"
   | CExchange => "CExchange"
   | CCAS => "CCAS"
+  | CFAA => "CFAA"
   | CPerf => "CPerf"
   | CResume => "CResume"
   | CWrap => "CWrap"
@@ -476,6 +479,7 @@ Fixpoint string_of_micro {A E} (ppa : A → string) (ppe : E → string) (m : mi
   | Stop CLoad loc k => "Stop(CLoad" ++ ", " ++ string_of_Z loc.(address) ++ ", <cont>)"
   | Stop CExchange (loc, v) k => "Stop(CExchange" ++ ", " ++ string_of_Z loc.(address) ++ ", " ++ string_of_val v ++ ", <cont>)"
   | Stop CCAS (loc, seen, v) k => "Stop(CCAS" ++ ", " ++ string_of_Z loc.(address) ++ ", " ++ string_of_val seen ++ ", " ++ string_of_val v ++ ", <cont>)"
+  | Stop CFAA (loc, i) k => "Stop(CFAA" ++ ", " ++ string_of_Z loc.(address) ++ ", " ++ string_of_int i ++ ", <cont>)"
   | Stop CPerf v k => "Stop(CPerf" ++ ", " ++ string_of_val v ++ ", <cont>)"
   | Stop CResume (loc, o2) k => "Stop(CResume" ++ ", " ++ string_of_Z loc.(address) ++ ", " ++ string_of_outcome2 o2 ++ ", <cont>)"
   | Stop CWrap (d, loc, η, h) k => "Stop(CWrap" ++ ", " ++ string_of_bool d ++ ", " ++ string_of_Z loc.(address) ++ "<env>, <handler>" ++ ", <cont>)"
